Instances/Store.v
@@ -3,23 +3,22 @@ Require Export Base.
 Require Import Classes.Monad Classes.Monad.MonadState 
   Types.State Classes.Galois Types.Option.
 
-Implicit Type ST : Type.
+Implicit Type S : Type.
 Implicit Type M : Type → Type.
-Generalizable Variables ST M.
 
-Instance store_state : MonadState ST (State ST) := {
+Instance store_state {S} : MonadState S (State S) := {
   get := λ st, (st, st);
   put := λ st, λ _, (tt, st);
 }.
 
-Instance get_store_state_sound {ST ST' : Type} {GS : Galois ST ST'} : 
-  get_state_sound (State ST) (State ST').
+Instance get_store_state_sound {S S' : Type} {GS : Galois S S'} : 
+  get_state_sound (State S) (State S').
 Proof.
   unfold get_state_sound. constructor; assumption.
 Qed.
 Hint Resolve get_store_state_sound : soundness.
 
-Instance store_stateT `{MM : Monad M} : MonadState ST (StateT ST M) := {
+Instance store_stateT {S} {M} {MM : Monad M} : MonadState S (StateT S M) := {
   get := λ st, returnM (st, st);
   put := λ st, λ _, returnM (tt, st);
 }.
@@ -67,41 +66,29 @@ Proof.
 Qed.
 Hint Resolve get_store_optionT_sound : soundness.
 
-
-Instance store_optionAT {ST M} {MM : Monad M} {MS : MonadState ST M} 
-  {JS : joinsecondable M} :
-  MonadState ST (optionAT M) := {
+Instance store_optionAT {S} {JS: Joinable S S} {JI : JoinableIdem JS} :
+  MonadState S (optionAT (StateT S option)) := {
   get := get >>= λ a, returnM (SomeA a);
   put := λ st, put st ;; returnM (SomeA tt);
 }.
 
-Instance get_store_optionAT_sound {ST ST' : Type} {GST : Galois ST ST'}
-  {M M' : Type → Type} {MM : Monad M} {MM' : Monad M'}
-  {JS : joinsecondable M}
-  {GM : ∀ A A', Galois A A' → Galois (M A) (M' A')}
-  {MS : MonadState ST M} {MS' : MonadState ST' M'} :
-  bind_sound M M' →
-  return_sound M M' →
-  get_state_sound M M' → 
-  get_state_sound (optionAT M) (optionT M').
+Instance get_store_optionAT_sound {S S' : Type} {GS : Galois S S'} 
+  {JS : Joinable S S} {JSI : JoinableIdem JS} :
+  get_state_sound (optionAT (StateT S option)) (optionT (StateT S' option)).
 Proof.
-  intros BS RS GS.
   unfold get_state_sound, get; simpl. 
-  eapply BS. auto. intros a a' Ha. eauto with soundness.
+  eauto with soundness.
 Qed.
 Hint Resolve get_store_optionAT_sound : soundness.
 
-Instance put_store_optionAT_sound {ST ST' : Type} {GST : Galois ST ST'}
-  {M M' : Type → Type} {MM : Monad M} {MM' : Monad M'}
-  {JS : joinsecondable M} 
-  {GM : ∀ A A', Galois A A' → Galois (M A) (M' A')}
-  {MS : MonadState ST M} {MS' : MonadState ST' M'} :
-  return_sound M M' →
-  bind_sound M M' →
-  put_state_sound M M' →
-  put_state_sound (optionAT M) (optionT M').
+Instance put_store_optionAT_sound {S S' : Type} {GS : Galois S S'}
+  {JS : Joinable S S} {JI : JoinableIdem JS} :
+  put_state_sound (optionAT (StateT S option)) (optionT (StateT S' option)).
 Proof.
-  intros RS BS PS s s' Hs. cbn. eapply BS.  apply PS. assumption.
-  intros ???. apply RS. constructor. constructor.
+  intros s s' Hs; cbn.
+  unfold bindM; simpl; unfold bind_stateT.
+  intros s2 s2' Hs2.
+  unfold bindM; simpl; unfold bind_option.
+  constructor. constructor; eauto with soundness.
 Qed.
 Hint Resolve put_store_optionAT_sound : soundness.
